Relax linking constraints

doc/coq/Abstract.v
@@ -2,17 +2,17 @@ From MODULAR Require Export Syntax.
 
 Generalizable Variables T.
 
-Inductive state {time : Type} :=
-  | ST (mem : time -> list (@expr_value time))
-       (t : time)
+Inductive state {T : Type} :=
+  | ST (mem : T -> list (@expr_value T))
+       (t : T)
 .
 
-Class Time `{OrderT T} :=
+Class time `{OrderT T} :=
 {  
   update : (@dy_ctx T) -> (@state T) -> expr_id -> (@expr_value T) -> T;
 }.
 
-Definition update_m {X} `{Time T} mem (t : T) (x : X) :=
+Definition update_m {X} `{time T} mem (t : T) (x : X) :=
   fun t' => 
   if eqb t' t then
     x :: (mem t)
@@ -23,7 +23,7 @@ Definition empty_mem {X T} (t : T) : list X := [].
 Notation "p '!#->' v ';' mem" := (update_m mem p v)
                               (at level 100, v at next level, right associativity).
 
-Inductive EvalR `{Time T} (C : @dy_ctx T) (st : @state T)
+Inductive EvalR `{time T} (C : @dy_ctx T) (st : @state T)
     : tm -> dy_value -> state -> Prop :=
   | Eval_var_e x v mem t addr
              (STATE : ST mem t = st)
@@ -48,10 +48,10 @@ Inductive EvalR `{Time T} (C : @dy_ctx T) (st : @state T)
     : EvalR C st (e_app e1 e2) (EVal v) st_v
   | Eval_link m e C_m st_m v st_v
               (MOD : EvalR C st m (MVal C_m) st_m)
-              (LINK : EvalR C_m st_m e (EVal v) st_v)
-    : EvalR C st (e_link m e) (EVal v) st_v
+              (LINK : EvalR C_m st_m e v st_v)
+    : EvalR C st (e_link m e) v st_v
   | Eval_empty
-    : EvalR C st m_empty (MVal ([||])) st
+    : EvalR C st m_empty (MVal C) st
   | Eval_var_m M C_M (ACCESS : Some C_M = ctx_M C M)
     : EvalR C st (m_var M) (MVal C_M) st
   | Eval_lete x e v mem t
@@ -61,19 +61,19 @@ Inductive EvalR `{Time T} (C : @dy_ctx T) (st : @state T)
                         (ST (t !#-> v ; mem) 
                             (update C (ST mem t) x v))
                         m (MVal C_m) st_m)
-    : EvalR C st (m_lete x e m) (MVal (dy_c_lete x t C_m)) st_m
+    : EvalR C st (m_lete x e m) (MVal C_m) st_m
   | Eval_letm M m' C' st'
               m'' C'' st''
               (EVALm' : EvalR C st m' (MVal C') st')
               (EVALm'' : EvalR (C [|dy_c_letm M C' ([||])|]) st'
                          m'' (MVal C'') st'')
-    : EvalR C st (m_letm M m' m'') (MVal (dy_c_letm M C' C'')) st''
+    : EvalR C st (m_letm M m' m'') (MVal C'') st''
 .
 
 #[export] Hint Constructors EvalR : core.
 
 (* Reachability relation *)
-Inductive ReachR `{Time T} (C : dy_ctx) (st : state)
+Inductive ReachR `{time T} (C : dy_ctx) (st : state)
     : tm -> (@dy_ctx T) -> (@state T) -> tm -> Prop :=
   | r_refl e
     : ReachR C st e 
@@ -150,7 +150,7 @@ Notation "'<|' C1 st1 tm1 '~#>' C2 st2 tm2 '|>'" := (ReachR C1 st1 tm1 C2 st2 tm
                                                 C2 at next level, st2 at next level, tm2 at next level).
 
 (* sanity check *)
-Lemma reach_trans : forall `{Time T} (C1 : @dy_ctx T) st1 e1
+Lemma reach_trans : forall `{time T} (C1 : @dy_ctx T) st1 e1
                          C2 st2 e2
                          C3 st3 e3
                          (REACH1 : <| C1 st1 e1 ~#> C2 st2 e2 |>)
@@ -163,7 +163,7 @@ Proof.
 Qed.
 
 Lemma value_reach_only_itself_e :
-  forall `{Time T} (C : @dy_ctx T) st v (pf : value v)
+  forall `{time T} (C : @dy_ctx T) st v (pf : value v)
          C' st' e'
          (REACH : <| C st v ~#> C' st' e' |>),
          C = C' /\ st = st' /\ v = e'.
@@ -173,7 +173,7 @@ Proof.
 Qed.
 
 Lemma Meval_then_collect :
-  forall `{Time T} C st m v st_m
+  forall `{time T} C st m v st_m
          (EVAL : EvalR C st m v st_m)
          C_m (MVAL : v = MVal C_m),
         match collect_ctx (dy_to_st C) m with
@@ -183,6 +183,12 @@ Lemma Meval_then_collect :
 Proof.
   intros. rename H into H'. rename H0 into H0'. revert C_m MVAL.
   induction EVAL; intros; simpl; try inversion MVAL; subst; eauto.
+  - specialize (IHEVAL1 C_m eq_refl). 
+    specialize (IHEVAL2 C_m0 eq_refl). 
+    destruct (collect_ctx (dy_to_st C) m). destruct o.
+    rewrite <- IHEVAL1 in IHEVAL2.
+    destruct (collect_ctx s e). exact IHEVAL2. 
+    exact IHEVAL1.
   - pose proof (mod_is_static_some C M) as H.
     destruct H as [A B]. specialize (A C_m).
     symmetry in ACCESS. specialize (A ACCESS).
@@ -190,13 +196,13 @@ Proof.
   - rewrite dy_to_st_plugin in IHEVAL2.
     simpl in IHEVAL2.
     remember (collect_ctx (dy_to_st C [[|st_c_lete x ([[||]])|]]) m) as ol.
-    destruct ol. destruct o; eauto. erewrite IHEVAL2; simpl; eauto.
+    destruct ol. apply IHEVAL2; eauto.
   - rewrite dy_to_st_plugin in IHEVAL2. simpl in IHEVAL2.
-    specialize (IHEVAL1 C' eq_refl). specialize (IHEVAL2 C'' eq_refl).
+    specialize (IHEVAL1 C' eq_refl). specialize (IHEVAL2 C_m eq_refl).
     destruct (collect_ctx (dy_to_st C) m'). destruct o; try apply IHEVAL1.
     rewrite <- IHEVAL1 in IHEVAL2.
     destruct (collect_ctx (dy_to_st C [[|st_c_letm M s ([[||]])|]]) m'').
-    destruct o; eauto. rewrite IHEVAL1; rewrite IHEVAL2; simpl; eauto.
+    apply IHEVAL2.
 Qed.
 
 Definition ctx_bound_st {T} ub (st : @state T) :=
@@ -214,7 +220,7 @@ Definition ctx_bound_tm {T} ub (C : @dy_ctx T) (st : @state T) e :=
          In sC ub.
 
 Lemma eval_ctx_bound :
-  forall `{Time T} ub
+  forall `{time T} ub
          (C : @dy_ctx T) st e
          v st'
          (INIT : ctx_bound_tm ub C st e)
@@ -260,9 +266,9 @@ Proof.
   - apply IHEVAL2. clear IHEVAL2.
     simpl in B.
     assert (forall sC : st_ctx, In sC (snd (collect_ctx (dy_to_st C) m)) -> In sC ub).
-    { intros. destruct (collect_ctx (dy_to_st C) m). 
-      destruct o; specialize (B sC); apply B. 
-      rewrite in_app_iff. left; eauto. eauto. }
+    { intros. destruct (collect_ctx (dy_to_st C) m).
+      destruct o; try destruct (collect_ctx s e); apply B;
+      try rewrite in_app_iff; try left; eauto. }
     assert (ctx_bound_tm ub C st m). 
     { split; eauto. destruct (collect_ctx (dy_to_st C) m); eauto. }
     specialize (IHEVAL1 H0). clear H H0.
@@ -309,7 +315,7 @@ Proof.
 Qed.
 
 Lemma reach_ctx_bound :
-  forall `{Time T} ub
+  forall `{time T} ub
          (C : @dy_ctx T) st e
          C' st' e'
          (INIT : ctx_bound_tm ub C st e)
@@ -350,7 +356,7 @@ Proof.
     intros; apply B. simpl in *. rewrite in_app_iff. left; eauto.
   - split; eauto. simpl in B.
     destruct (collect_ctx (dy_to_st C) m). 
-    intros. destruct o; apply B; eauto.
+    intros. destruct o; try destruct (collect_ctx s e); apply B; eauto.
     rewrite in_app_iff. left; eauto.
   - eapply Meval_then_collect in MOD as MOD'; eauto.
     apply eval_ctx_bound with (ub := ub) in MOD.
@@ -361,7 +367,7 @@ Proof.
     intros; apply B; simpl; rewrite in_app_iff; right; eauto.
     split; eauto. simpl in B.
     destruct (collect_ctx (dy_to_st C) m). 
-    intros. destruct o; apply B; eauto.
+    intros. destruct o; try destruct (collect_ctx s e); apply B; eauto.
     rewrite in_app_iff. left; eauto.
   - split; eauto. simpl in B.
     destruct (collect_ctx (dy_to_st C) e).
@@ -402,7 +408,7 @@ Proof.
 Qed.
 
 Theorem expr_ctx_bound :
-  forall `{Time T} init e C' st' e'
+  forall `{time T} init e C' st' e'
          (REACH : <| ([||]) (ST empty_mem init) e ~#> C' st' e' |>),
          In (dy_to_st C') (snd (collect_ctx ([[||]]) e)).
 Proof.
