doc/coq/Linking.v
@@ -1,4 +1,5 @@
 From MODULAR Require Export Sound.
+Require Export Coq.Logic.FunctionalExtensionality.
 
 (* before, after *)
 Generalizable Variables BT AT.
@@ -102,17 +103,149 @@ Qed.
     eqb_neq := link_eqb_neq
   }.
 
-Definition filter_mem 
-  `{BO : OrderT BT} `{AO : OrderT AT} `{OrderT (@link )}
-  (mem : BT -> option (@expr_value BT)) := 1.
+Fixpoint filter_ctx_bf
+  `{BO : OrderT BT} `{AO : OrderT AT}
+  (C : @dy_ctx (@link BT BO AT AO)) :=
+  match C with
+  | ([||]) => ([||])
+  | dy_c_lam x t C' =>
+    match t with
+    | AF t => filter_ctx_bf C'
+    | BF t => dy_c_lam x t (filter_ctx_bf C')
+    end
+  | dy_c_lete x t C' =>
+    match t with
+    | AF t => filter_ctx_bf C'
+    | BF t => dy_c_lete x t (filter_ctx_bf C')
+    end
+  | dy_c_letm M C' C'' =>
+    dy_c_letm M (filter_ctx_bf C') (filter_ctx_bf C'')
+  end.
 
-Fixpoint inject_ctx `{OrderT T1}Cout Cin :=
+Fixpoint filter_ctx_af
+  `{BO : OrderT BT} `{AO : OrderT AT}
+  (C : @dy_ctx (@link BT BO AT AO)) :=
+  match C with
+  | ([||]) => ([||])
+  | dy_c_lam x t C' =>
+    match t with
+    | AF t => dy_c_lam x t (filter_ctx_af C')
+    | BF t => filter_ctx_af C'
+    end
+  | dy_c_lete x t C' =>
+    match t with
+    | AF t => dy_c_lete x t (filter_ctx_af C')
+    | BF t => filter_ctx_af C'
+    end
+  | dy_c_letm M C' C'' =>
+    dy_c_letm M (filter_ctx_af C') (filter_ctx_af C'')
+  end.
+
+Definition filter_mem_bf
+  `{BO : OrderT BT} `{AO : OrderT AT}
+  (mem : (@link BT BO AT AO) -> option (@expr_value (@link BT BO AT AO))) :=
+  fun t =>
+    match mem (BF t) with
+    | Some (Closure x e C) => Some (Closure x e (filter_ctx_bf C))
+    | None => None
+    end.
+
+Definition filter_mem_af
+  `{BO : OrderT BT} `{AO : OrderT AT}
+  (mem : (@link BT BO AT AO) -> option (@expr_value (@link BT BO AT AO))) :=
+  fun t =>
+    match mem (AF t) with
+    | Some (Closure x e C) => Some (Closure x e (filter_ctx_af C))
+    | None => None
+    end.
+
+Definition filter_v_bf 
+  `{BO : OrderT BT} `{AO : OrderT AT}
+  (v : @expr_value (@link BT BO AT AO)) :=
+  match v with
+  | Closure x e C => Closure x e (filter_ctx_bf C)
+  end.
+
+Definition filter_v_af
+  `{BO : OrderT BT} `{AO : OrderT AT}
+  (v : @expr_value (@link BT BO AT AO)) :=
+  match v with
+  | Closure x e C => Closure x e (filter_ctx_af C)
+  end.
+
+Definition link_update
+  `{Conc.time BT} `{Conc.time AT}
+  (C : @dy_ctx link) (st : @state link) x v :=
+  match st with
+  | ST mem (BF t) =>
+    BF (update (filter_ctx_bf C) (ST (filter_mem_bf mem) t) x (filter_v_bf v))
+  | ST mem (AF t) =>
+    AF (update (filter_ctx_af C) (ST (filter_mem_af mem) t) x (filter_v_af v))
+  end.
+
+Lemma link_update_lt :
+  forall `{Conc.time BT} `{Conc.time AT}
+         C mem t x v, 
+  let t' := link_update C (ST mem t) x v in
+  link_leb t t' = true /\ link_eqb t t' = false.
+Proof.
+  intros. destruct t; simpl in *; try apply update_lt.
+Qed.
+
+#[export] Instance link_time `{Conc.time BT} `{Conc.time AT} : (@Conc.time link LinkOrderT) :=
+{
+  update := link_update;
+  update_lt := link_update_lt
+}.
+
+Fixpoint lift_ctx_bf `{OrderT BT} (C : @dy_ctx BT) :=
+  match C with
+  | ([||]) => ([||])
+  | dy_c_lam x t C' => dy_c_lam x (BF t) (lift_ctx_bf C')
+  | dy_c_lete x t C' => dy_c_lete x (BF t) (lift_ctx_bf C')
+  | dy_c_letm M C' C'' => dy_c_letm M (lift_ctx_bf C') (lift_ctx_bf C'')
+  end.
+
+Fixpoint lift_ctx_af `{OrderT AT} (C : @dy_ctx AT) :=
+  match C with
+  | ([||]) => ([||])
+  | dy_c_lam x t C' => dy_c_lam x (AF t) (lift_ctx_af C')
+  | dy_c_lete x t C' => dy_c_lete x (AF t) (lift_ctx_af C')
+  | dy_c_letm M C' C'' => dy_c_letm M (lift_ctx_af C') (lift_ctx_af C'')
+  end.
+
+Fixpoint inject_ctx {T} (Cout : @dy_ctx T) (Cin : @dy_ctx T) :=
   match Cin with
   | ([||]) => Cout
   | dy_c_lam x t C' =>
     inject_ctx (Cout [|dy_c_lam x t ([||])|]) C'
   | dy_c_lete x t C' =>
     inject_ctx (Cout [|dy_c_lete x t ([||])|]) C'
-  | dy_c_letm M CM C' => 
-    inject_ctx (Cout [|dy_c_letm M (inject_ctx Cout CM) ([||])|]) C'
+  | dy_c_letm M C' C'' => 
+    inject_ctx (Cout [|dy_c_letm M (inject_ctx Cout C') ([||])|]) C''
   end.
+
+Notation "Cout '<|' Cin '|>'" := (inject_ctx Cout Cin)
+                              (at level 100, Cin at next level, right associativity).
+
+Fixpoint lift_state_bf `{OrderT BT} (st : @state BT) :=
+  match C with
+  | ([||]) => ([||])
+  | dy_c_lam x t C' => dy_c_lam x (BF t) (lift_ctx_bf C')
+  | dy_c_lete x t C' => dy_c_lete x (BF t) (lift_ctx_bf C')
+  | dy_c_letm M C' C'' => dy_c_letm M (lift_ctx_bf C') (lift_ctx_bf C'')
+  end.
+
+Fixpoint lift_state_af `{OrderT AT} (st : @state AT) :=
+  match C with
+  | ([||]) => ([||])
+  | dy_c_lam x t C' => dy_c_lam x (AF t) (lift_ctx_af C')
+  | dy_c_lete x t C' => dy_c_lete x (AF t) (lift_ctx_af C')
+  | dy_c_letm M C' C'' => dy_c_letm M (lift_ctx_af C') (lift_ctx_af C'')
+  end.
+
+Definition inject_state {T} (st_out : @Conc.state T)
+
+Lemma link_eval `{Conc.time BT} `{Conc.time AT} :
+  forall (Cout : @dy_ctx BT) (Cin : @dy_ctx AT) st e e' st'
+         (EVAL : EvalR C st e e' st')
