doc/coq/Sound.v
@@ -7,12 +7,12 @@ Module Conc := Concrete.
 Generalizable Variables CT.
 Generalizable Variables AT.
 
-Definition lt `{Conc.Time CT} (t1 : CT) (t2 : CT) :=
+Definition lt `{Conc.time CT} (t1 : CT) (t2 : CT) :=
   leb t1 t2 = true /\ eqb t1 t2 = false.
 
 Notation "t1 '<' t2" := (lt t1 t2).
 
-Fixpoint dy_ctx_bound `{Conc.Time CT} C t :=
+Fixpoint dy_ctx_bound `{Conc.time CT} C t :=
   match C with
   | [||] => True
   | dy_c_lam _ t' C'
@@ -20,7 +20,7 @@ Fixpoint dy_ctx_bound `{Conc.Time CT} C t :=
   | dy_c_letm _ CM C' => dy_ctx_bound CM t /\ dy_ctx_bound C' t
   end.
 
-Definition time_bound `{Conc.Time CT} C st :=
+Definition time_bound `{Conc.time CT} C st :=
   match st with
   | ST mem t =>
     dy_ctx_bound C t /\
@@ -34,7 +34,7 @@ Definition time_bound `{Conc.Time CT} C st :=
   end.
 
 Lemma p_bound_or_not :
-  forall `{Conc.Time CT} (p : CT) t,
+  forall `{Conc.time CT} (p : CT) t,
     (p < t) \/ ~(p < t).
 Proof.
   intros. unfold "<". unfold not.
@@ -48,10 +48,10 @@ Proof.
 Qed.
 
 Definition eq_bound_α 
-  `{Conc.Time CT} `{Abs.Time AT} t (α : CT -> AT) α' :=
+  `{Conc.time CT} `{Abs.time AT} t (α : CT -> AT) α' :=
   forall t' (LE : leb t' t = true), α t' = α' t'.
 
-Fixpoint trans_ctx `{Conc.Time CT} `{Abs.Time AT} (α : CT -> AT) C :=
+Fixpoint trans_ctx `{Conc.time CT} `{Abs.time AT} (α : CT -> AT) C :=
   match C with
   | [||] => [||]
   | dy_c_lam x t C' => dy_c_lam x (α t) (trans_ctx α C')
@@ -59,7 +59,7 @@ Fixpoint trans_ctx `{Conc.Time CT} `{Abs.Time AT} (α : CT -> AT) C :=
   | dy_c_letm M CM C' => dy_c_letm M (trans_ctx α CM) (trans_ctx α C')
   end.
 
-Definition sound `{Conc.Time CT} `{Abs.Time AT} α C st abs_C abs_st :=
+Definition sound `{Conc.time CT} `{Abs.time AT} α C st abs_C abs_st :=
   match abs_st with
   | Abs.ST abs_mem abs_t =>
     match st with
@@ -77,7 +77,7 @@ Definition sound `{Conc.Time CT} `{Abs.Time AT} α C st abs_C abs_st :=
   end.
 
 Lemma trans_ctx_addr :
-  forall `{Conc.Time CT} `{Abs.Time AT} α C x,
+  forall `{Conc.time CT} `{Abs.time AT} α C x,
     addr_x (trans_ctx α C) x = 
       match (addr_x C x) with 
       | None => None 
@@ -96,12 +96,12 @@ Proof.
 Qed.
 
 Lemma trans_ctx_ctx_M :
-  forall `{Conc.Time CT} `{Abs.Time AT} C α abs_C M C_M
+  forall `{Conc.time CT} `{Abs.time AT} C α abs_C M C_M
         (ACCESS : ctx_M C M = Some C_M)
         (TRANS : trans_ctx α C = abs_C),
     ctx_M abs_C M = Some (trans_ctx α C_M).
 Proof.
-  assert (forall `{Conc.Time CT} `{Abs.Time AT} C α M,
+  assert (forall `{Conc.time CT} `{Abs.time AT} C α M,
     match ctx_M (trans_ctx α C) M with
     | Some _ => 
       match ctx_M C M with
@@ -144,7 +144,7 @@ Proof.
 Qed.
 
 Lemma time_increase_e :
-  forall `{Conc.Time CT} `{Abs.Time AT} C st e e' st'
+  forall `{Conc.time CT} `{Abs.time AT} C st e e' st'
          (EVAL : EvalR C st e e' st'),
     match st with
     | ST _ t =>
@@ -175,7 +175,7 @@ Proof.
 Qed.
 
 Lemma relax_ctx_bound :
-  forall `{Conc.Time CT} `{Abs.Time AT} 
+  forall `{Conc.time CT} `{Abs.time AT} 
          C t1 t2 (BOUND : dy_ctx_bound C t1) (LE : leb t1 t2 = true),
          dy_ctx_bound C t2.
 Proof.
@@ -188,7 +188,7 @@ Proof.
 Qed.
 
 Lemma relax_p_bound :
-  forall `{Conc.Time CT} `{Abs.Time AT}
+  forall `{Conc.time CT} `{Abs.time AT}
     p t1 t2 (BOUND : p < t1) (LE : leb t1 t2 = true),
   p < t2.
 Proof.
@@ -201,7 +201,7 @@ Proof.
 Qed.
 
 Lemma time_bound_addr :
-  forall `{Conc.Time CT} `{Abs.Time AT} C x t,
+  forall `{Conc.time CT} `{Abs.time AT} C x t,
     dy_ctx_bound C t -> 
     match addr_x C x with
     | None => True
@@ -219,7 +219,7 @@ Proof.
 Qed.
 
 Lemma time_bound_ctx_M :
-  forall `{Conc.Time CT} `{Abs.Time AT} C M t CM,
+  forall `{Conc.time CT} `{Abs.time AT} C M t CM,
     ctx_M C M = Some CM ->
     dy_ctx_bound C t -> 
     dy_ctx_bound CM t.
@@ -237,7 +237,7 @@ Proof.
 Qed.
 
 Lemma plugin_ctx_bound :
-  forall `{Conc.Time CT} `{Abs.Time AT} Cout Cin t,
+  forall `{Conc.time CT} `{Abs.time AT} Cout Cin t,
     dy_ctx_bound (Cout[|Cin|]) t <-> dy_ctx_bound Cout t /\ dy_ctx_bound Cin t.
 Proof.
   intros. 
@@ -254,45 +254,8 @@ Proof.
   rewrite IHCout2; eauto.
 Qed.
 
-
-Ltac contradict :=
-  let contra := fresh "contra" in
-  assert False as contra; eauto 3; inversion contra.
-
-Lemma __R__ : forall b, b = false <-> ~ b = true.
-Proof. 
-  intros; destruct b; unfold "<>"; split; 
-  intros; try inversion H; try inversion H0; try contradict; eauto.
-Qed.
-
-Ltac refl_bool :=
-  let contra := fresh "contra" in
-  match goal with
-  | |- _ = false => 
-    rewrite __R__; unfold "<>"; intros contra
-  | |- _ <> true => 
-    rewrite <- __R__
-  | _ => idtac
-  end.
-
-Ltac lebt x :=
-  apply leb_trans with (t' := x); try assumption; try apply update_lt.
-
-Lemma eqb_refl : forall `{OrderT CT} t, eqb t t = true.
-Proof.
-  intros. rewrite eqb_eq. eauto.
-Qed.
-
-Lemma eqb_update : forall `{Conc.Time CT} C mem t x x' e' C',
-  eqb t (update C (ST mem t) x (Closure x' e' C')) = false.
-Proof.
-  intros. refl_bool.
-  assert (t < update C (ST mem t) x (Closure x' e' C')) as contra'. apply update_lt.
-  destruct contra' as [? contra']. rewrite contra' in *. inversion contra.
-Qed.
-
 Lemma time_bound_e :
-  forall `{Conc.Time CT} `{Abs.Time AT} C st e e' st'
+  forall `{Conc.time CT} `{Abs.time AT} C st e e' st'
          (EVAL : EvalR C st e e' st')
          (BOUND : time_bound C st),
     match e' with
@@ -357,10 +320,7 @@ Proof.
       specialize (H1 p contra). rewrite H1 in ACCESS. inversion ACCESS. apply H.
   - apply IHEVAL2. apply IHEVAL1. eauto.
   - destruct st. simpl in *. destruct BOUND as [? [? ?]].
-    repeat split; eauto.
-  - destruct st. simpl in *. destruct BOUND as [? [? ?]].
-    repeat split; eauto.
-    eapply time_bound_ctx_M.
+    repeat split; eauto. eapply time_bound_ctx_M.
     symmetry. exact ACCESS. eauto.
   - specialize (IHEVAL1 BOUND).
     destruct v. 
@@ -369,61 +329,39 @@ Proof.
     apply time_increase_e in EVAL2 as time_inc2.
     simpl in BOUND. destruct BOUND as [B1 [B2 B3]].
     simpl in IHEVAL1. destruct IHEVAL1 as [HH1 [HH2 HH3]].
-    assert (time_bound C_m (ST mem1 t1)).
-    {
-      apply IHEVAL2.
-      simpl; rewrite plugin_ctx_bound. split. split.
-      apply relax_ctx_bound with (t1 := t0); try assumption. 
-      lebt t. simpl. split; eauto; try apply update_lt.
-      split; intros; unfold update_m; remember (eqb p t) as b;
-      destruct b; symmetry in Heqb; try rewrite eqb_eq in Heqb; try rewrite eqb_neq in Heqb.
-      - subst. assert False as contra. apply NBOUND. apply update_lt. inversion contra.
-      - apply HH2. unfold not. intros. 
-        assert False as contra. apply NBOUND.
-        apply relax_p_bound with (t1 := t); try assumption. apply update_lt. eauto.
-      - subst. apply relax_ctx_bound with (t1 := t); try assumption. apply update_lt.
-      - specialize (HH3 p). remember (mem p) as access eqn:ACCESS.
-        destruct access; eauto. destruct e1.
-        apply relax_ctx_bound with (t1 := t); try assumption. apply HH3.
-        pose proof (p_bound_or_not p t) as CASES.
-        destruct CASES as [? | contra]; eauto.
-        specialize (HH2 p contra). rewrite HH2 in ACCESS. inversion ACCESS. apply update_lt.
-    }
-    destruct H as [HH1' [HH2' HH3']].
-    repeat split; try assumption.
-    lebt ((update C (ST mem t) x (Closure x0 e0 C0))).
-    refl_bool. rewrite eqb_eq in contra. rewrite contra in time_inc2. clear contra.
-    assert (t1 = (update C (ST mem t1) x (Closure x0 e0 C0))).
-    apply leb_sym; try assumption. apply update_lt.
-    assert (eqb t1 (update C (ST mem t1) x (Closure x0 e0 C0)) = false) as contra.
-    apply update_lt.
-    rewrite eqb_neq in contra. apply contra; eauto.
+    apply IHEVAL2. simpl; split.
+    rewrite plugin_ctx_bound; split.
+    apply relax_ctx_bound with (t1 := t0); eauto. 
+    apply leb_trans with (t' := t); try assumption. apply update_lt. 
+    simpl; split; eauto. apply update_lt.
+    split; intros;
+    unfold update_m; remember (eqb p t) as b;
+    destruct b; symmetry in Heqb; try rewrite eqb_eq in Heqb.
+    + subst. assert False as contra. apply NBOUND. apply update_lt. inversion contra.
+    + apply HH2. unfold not. intros. 
+      assert False as contra. apply NBOUND.
+      apply relax_p_bound with (t1 := t); try assumption. apply update_lt. eauto.
+    + subst. apply relax_ctx_bound with (t1 := t); try assumption. apply update_lt.
+    + specialize (HH3 p). remember (mem p) as access eqn:ACCESS.
+      destruct access; eauto. destruct e1.
+      apply relax_ctx_bound with (t1 := t); try assumption. apply HH3.
+      pose proof (p_bound_or_not p t) as CASES.
+      destruct CASES as [? | contra]; eauto.
+      specialize (HH2 p contra). rewrite HH2 in ACCESS. inversion ACCESS. apply update_lt.
   - specialize (IHEVAL1 BOUND).
     destruct st. destruct st'. destruct st''.
     simpl in BOUND. destruct BOUND as [B1 [B2 B3]].
     simpl in IHEVAL1. destruct IHEVAL1 as [HH1 [HH2 HH3]].
     apply time_increase_e in EVAL1 as time_inc1.
     apply time_increase_e in EVAL2 as time_inc2.
-    assert (time_bound C'' (ST mem1 t1)).
-    {
-      apply IHEVAL2.
-      simpl; rewrite plugin_ctx_bound. split. split.
-      apply relax_ctx_bound with (t1 := t); try assumption. 
-      simpl. split; eauto.
-      split; intros; unfold update_m; remember (eqb p t) as b;
-      destruct b; symmetry in Heqb; try rewrite eqb_eq in Heqb; try rewrite eqb_neq in Heqb.
-      - apply HH2; eauto.
-      - apply HH2; eauto.
-      - apply HH3; eauto.
-      - apply HH3; eauto.
-    }
-    destruct H as [HH1' [HH2' HH3']].
-    repeat split; try assumption.
-    apply relax_ctx_bound with (t1 := t0); eauto.
+    apply IHEVAL2. simpl. repeat split; eauto.
+    rewrite plugin_ctx_bound. split.
+    apply relax_ctx_bound with (t1 := t); eauto.
+    simpl; split; eauto.
 Qed.
 
 Lemma plugin_trans_ctx :
-  forall `{Conc.Time CT} `{Abs.Time AT} Cout Cin α,
+  forall `{Conc.time CT} `{Abs.time AT} Cout Cin α,
     trans_ctx α (Cout[|Cin|]) = (trans_ctx α Cout [|trans_ctx α Cin|]).
 Proof.
   induction Cout; intros; simpl; 
@@ -432,7 +370,7 @@ Proof.
 Qed.
 
 Lemma bound_trans_ctx_eq :
-  forall `{Conc.Time CT} `{Abs.Time AT} C t α α',
+  forall `{Conc.time CT} `{Abs.time AT} C t α α',
          dy_ctx_bound C t ->
          eq_bound_α t α α' ->
          trans_ctx α C = trans_ctx α' C.
@@ -447,10 +385,43 @@ Proof.
   unfold eq_bound_α in H0. rewrite H4; eauto.
 Qed.
 
+Ltac contradict :=
+  let contra := fresh "contra" in
+  assert False as contra; eauto 3; inversion contra.
+
+Lemma __R__ : forall b, b = false <-> ~ b = true.
+Proof. 
+  intros; destruct b; unfold "<>"; split; 
+  intros; try inversion H; try inversion H0; try contradict; eauto.
+Qed.
+
+Ltac refl_bool :=
+  match goal with
+  | |- _ = false => rewrite __R__
+  | |- _ <> true => rewrite <- __R__
+  | _ => idtac
+  end.
+
+Ltac lebt x :=
+  apply leb_trans with (t' := x); try assumption; try apply update_lt.
+
+Lemma eqb_refl : forall `{OrderT CT} t, eqb t t = true.
+Proof.
+  intros. rewrite eqb_eq. eauto.
+Qed.
+
+Lemma eqb_update : forall `{Conc.time CT} C mem t x x' e' C',
+  eqb t (update C (ST mem t) x (Closure x' e' C')) = false.
+Proof.
+  intros. refl_bool. unfold "<>". intros.
+  assert (t < update C (ST mem t) x (Closure x' e' C')) as contra. apply update_lt.
+  destruct contra as [? contra]. rewrite contra in *. inversion H1.
+Qed.
+
 (* Set Printing Implicit. *)
 
 Lemma sound_eval :
-  forall `{Conc.Time CT} `{Abs.Time AT} C st e v' st'
+  forall `{Conc.time CT} `{Abs.time AT} C st e v' st'
          (EVAL : EvalR C st e v' st')
          (BOUND : time_bound C st)
          abs_C abs_st α
@@ -525,7 +496,7 @@ Proof.
       assert False as contra. apply NBOUND. apply update_lt. inversion contra.
       apply BB2''. unfold not. intros [LE NEQ].
       apply NBOUND. split. lebt t.
-      refl_bool. rewrite eqb_eq in *.
+      refl_bool. unfold "<>". intros contra. rewrite eqb_eq in *.
       assert (t = p) as RR. apply leb_sym; try assumption. rewrite contra. apply update_lt.
       rewrite eqb_neq in NEQ. apply NEQ; eauto.
       (* bound, then access is bound *)
@@ -556,7 +527,7 @@ Proof.
     assert (eq_bound_α t α'' α''') as EQ'''.
     { red. intros. rewrite Heqα'''. 
       assert (eqb t' (update C (ST mem t) x (Closure x0 e0 C0)) = false) as RR.
-      refl_bool. rewrite eqb_eq in contra.
+      refl_bool. unfold "<>". intros contra. rewrite eqb_eq in contra.
       assert (leb t t' = true). rewrite contra. apply update_lt. 
       assert (t = t') as RR. apply leb_sym; eauto. rewrite <- RR in contra.
       clear RR.
@@ -577,7 +548,7 @@ Proof.
         destruct abs_st'. simpl in SOUND'. destruct SOUND' as [[? [? ?]] ?]. rewrite <- H0.
         apply bound_trans_ctx_eq with (t := t1). apply BOUND'.
         red. intros. assert (eqb t' (update C (ST mem t) x (Closure x0 e0 C0)) = false).
-        refl_bool. rewrite eqb_eq in contra.
+        refl_bool. unfold "<>". intros contra. rewrite eqb_eq in contra.
         assert (leb t' t = true). lebt t1.
         assert (t = t') as RR. apply leb_sym; try assumption. rewrite contra. apply update_lt.
         assert (t < t') as contra'. rewrite contra. apply update_lt.
@@ -631,9 +602,9 @@ Proof.
     rewrite RR. simpl in SOUND''. destruct SOUND'' as [? [RR' ?]].
     rewrite RR'. rewrite <- H2. rewrite <- H2 in EVAL'''. exact EVAL'''.
   - pose proof (time_bound_e C st m (MVal C_m) st_m EVAL1) as BOUND'.
-    pose proof (time_bound_e C_m st_m e (EVal v) st_v EVAL2) as BOUND''.
+    pose proof (time_bound_e C_m st_m e v st_v EVAL2) as BOUND''.
     specialize (BOUND' BOUND). simpl in BOUND'. 
-    specialize (BOUND'' BOUND'). simpl in BOUND''. destruct v.
+    specialize (BOUND'' BOUND'). simpl in BOUND''. (* destruct v. destruct ev. *)
     destruct st. destruct st_m. destruct st_v.
     apply time_increase_e in EVAL1 as time_inc1.
     apply time_increase_e in EVAL2 as time_inc2.
@@ -642,18 +613,19 @@ Proof.
     destruct SOUND' as [SOUND' EVAL']. 
     specialize (IHEVAL2 BOUND' abs_C' abs_st' α' SOUND').
     destruct IHEVAL2 as [abs_C'' [abs_st'' [α'' [EQ'' SOUND'']]]].
-    destruct SOUND'' as [SOUND'' EVAL''].
-    exists abs_C''. exists abs_st''. exists α''. repeat split; eauto.
-    unfold eq_bound_α in *. intros.
-    assert (α'' t' = α' t'). symmetry. apply EQ''. lebt t.
-    rewrite H. apply EQ'. eauto.
-    eapply Abstract.Eval_link. eauto.
-    destruct abs_st'. simpl in SOUND'. destruct SOUND' as [? [RR ?]].
-    rewrite RR. eauto.
-  - exists ([||]). exists abs_st. exists α. destruct st.
+    destruct v; try destruct ev;
+    destruct SOUND'' as [SOUND'' EVAL''];
+    exists abs_C''; exists abs_st''; exists α''; repeat split; eauto;
+    unfold eq_bound_α in *; intros;
+    try assert (α'' t' = α' t'); try symmetry; try apply EQ''; try lebt t;
+    try (rewrite H; symmetry; apply EQ'; eauto);
+    eapply Abstract.Eval_link; eauto;
+    destruct abs_st'; simpl in SOUND'; destruct SOUND' as [? [RR ?]];
+    rewrite RR; eauto.
+  - exists abs_C. exists abs_st. exists α. destruct st.
     repeat split; eauto. unfold eq_bound_α; intros; eauto.
     destruct abs_st. simpl in SOUND. destruct SOUND as [? [RR ?]].
-    simpl. repeat split; eauto.
+    rewrite RR. eauto.
   - exists (trans_ctx α C_M). exists abs_st. exists α. destruct st.
     destruct abs_st. destruct SOUND as [? [RR ?]].
     repeat split; eauto. rewrite <- RR.
@@ -680,7 +652,7 @@ Proof.
       assert False as contra. apply NBOUND. rewrite Heqb. apply update_lt. inversion contra.
       apply BB2'. unfold not. intros [LE NEQ].
       apply NBOUND. split. lebt t.
-      refl_bool. unfold "<>". rewrite eqb_eq in *.
+      refl_bool. unfold "<>". intros contra. rewrite eqb_eq in *.
       assert (t = p) as RR. apply leb_sym; try assumption. rewrite contra. apply update_lt.
       rewrite eqb_neq in NEQ. apply NEQ; eauto.
       (* bound, then access is bound *)
@@ -706,7 +678,7 @@ Proof.
     assert (eq_bound_α t α' α'') as EQ''.
     { red. intros. rewrite Heqα''. 
       assert (eqb t'0 (update C (ST mem t) x (Closure x0 e0 C0)) = false).
-      refl_bool. rewrite eqb_eq in contra.
+      refl_bool. unfold "<>". intros contra. rewrite eqb_eq in contra.
       assert (leb t t'0 = true). rewrite contra. apply update_lt. 
       assert (t = t'0) as RR. apply leb_sym; eauto. rewrite <- RR in contra.
       clear RR.
@@ -728,7 +700,7 @@ Proof.
         simpl in SOUND. destruct SOUND as [? [RR ?]]. rewrite <- RR. symmetry.
         apply bound_trans_ctx_eq with (t := t0). destruct BOUND. eauto.
         red. intros. rewrite Heqα''. assert (eqb t'0 (update C (ST mem t) x (Closure x0 e0 C0)) = false).
-        refl_bool. rewrite eqb_eq in contra.
+        refl_bool. unfold "<>". intros contra. rewrite eqb_eq in contra.
         assert (leb t'0 t = true). lebt t0.
         assert (t = t'0) as RR'. apply leb_sym; try assumption. rewrite contra. apply update_lt.
         assert (t < t'0) as contra'. rewrite contra. apply update_lt.
@@ -770,22 +742,16 @@ Proof.
     destruct IHEVAL2 as [abs_C'' [abs_st'' [α''' [EQ''' SOUND''']]]].
     destruct SOUND' as [SOUND' EVAL'].
     destruct SOUND''' as [SOUND''' EVAL'''].
-    exists (dy_c_lete x (α''' t) abs_C''). exists abs_st''. exists α'''. repeat split.
+    exists abs_C''. exists abs_st''. exists α'''. repeat split; eauto.
     red. intros. 
     assert (α t'0 = α' t'0) as RR. apply EQ'. eauto. rewrite RR; clear RR.
     assert (α' t'0 = α'' t'0) as RR. apply EQ''. lebt t0. rewrite RR; clear RR.
     apply EQ'''. lebt t. lebt t0.
-    destruct abs_st''. simpl. repeat split; try apply SOUND'''.
-    assert (trans_ctx α''' C_m = abs_C'') as RR.
-    apply SOUND'''. rewrite RR. eauto.
-    assert (α''' t = t'') as RR.
-    { destruct SOUND' as [R ?]. rewrite <- R.
-      assert (α' t = α'' t) as RR. apply EQ''. apply leb_refl. rewrite RR; clear RR.
-      symmetry. apply EQ'''. apply update_lt. }
-    eapply Abstract.Eval_lete; rewrite RR.
-    exact EVAL'. 
-    destruct SOUND' as [RR' [RR'' ?]]. rewrite RR' in EVAL'''.
-    rewrite RR''. exact EVAL'''.
+    eapply Abstract.Eval_lete; eauto.
+    destruct SOUND' as [? [RR ?]]. rewrite RR. 
+    destruct abs_st''. destruct SOUND''' as [? [RR' ?]]. rewrite RR' in *.
+    rewrite <- H. rewrite <- H in EVAL'''.
+    rewrite <- RR in *. exact EVAL'''.
   - pose proof (time_bound_e C st m' (MVal C') st' EVAL1) as BOUND'.
     pose proof (time_bound_e (C [|dy_c_letm M C' ([||])|]) st' m''
                              (MVal C'') st'' EVAL2) as BOUND''.
@@ -825,17 +791,12 @@ Proof.
     destruct IHEVAL2 as [abs_C'' [abs_st'' [α'' [EQ''' SOUND''']]]].
     destruct SOUND' as [SOUND' EVAL'].
     destruct SOUND''' as [SOUND''' EVAL'''].
+    exists abs_C''. exists abs_st''. exists α''. repeat split; eauto.
+    red. intros. 
+    assert (α t' = α' t') as RR. apply EQ'. eauto. rewrite RR; clear RR.
+    apply EQ'''. lebt t.
+    eapply Abstract.Eval_letm; eauto.
     destruct abs_st'. destruct SOUND' as [? [RR ?]].
     destruct abs_st''. destruct SOUND''' as [? [RR' ?]].
-    assert (trans_ctx α' C' = trans_ctx α'' C') as RR''. 
-    { apply bound_trans_ctx_eq with (t := t0). apply BOUND'. assumption. }
-    exists (dy_c_letm M abs_C' abs_C''). exists (Abs.ST mem3 t3). exists α''. repeat split; eauto.
-    red. intros. 
-    assert (α t' = α' t') as RR'''. apply EQ'. eauto. rewrite RR'''.
-    apply EQ'''. lebt t.
-    simpl. rewrite <- RR''. rewrite RR'. rewrite RR. eauto.
-    eapply Abstract.Eval_letm.
-    rewrite <- RR in *. rewrite <- RR' in *. rewrite RR'' in *.
-    exact EVAL'.
-    rewrite <- RR in *. rewrite RR'' in *. exact EVAL'''.
+    rewrite RR in *. rewrite RR' in *. eauto.
 Qed.
